code/experimental/hash/Hacl.Hash.SHA2.Lemmas.fst
@@ -1,0 +1,54 @@
+module Hacl.Hash.SHA2.Lemmas
+
+open FStar.Mul
+open FStar.Ghost
+open FStar.HyperStack
+open FStar.ST
+open FStar.Buffer
+
+open C.Loops
+
+open Hacl.Cast
+open Hacl.UInt8
+open Hacl.UInt32
+open FStar.UInt32
+
+
+let lemma_aux_0 (t:UInt32.t{UInt32.v t >= 16 /\ UInt32.v t < 64}) : Lemma
+  (UInt32.v (t -^ 16ul) >= 0 /\ UInt32.v (t -^ 15ul) >= 0
+   /\ UInt32.v (t -^ 7ul) >= 0 /\ UInt32.v (t -^ 2ul) >= 0
+   /\ UInt32.v (t -^ 16ul) < 64 /\ UInt32.v (t -^ 15ul) < 64
+   /\ UInt32.v (t -^ 7ul) < 64 /\ UInt32.v (t -^ 2ul) < 64)
+  = ()
+
+
+#reset-options "--max_fuel 0 --max_ifuel 0 --z3rlimit 200"
+
+val lemma_ws_def_0: (b:Spec.SHA2.block_w) -> (t:Spec.SHA2.counter{t < 16}) -> Lemma
+  (Spec.SHA2.ws b t = Seq.index b t)
+#reset-options "--initial_fuel 1 --max_fuel 1 --z3rlimit 20"
+let lemma_ws_def_0 b t = ()
+
+
+#reset-options "--max_fuel 0 --max_ifuel 0 --z3rlimit 200"
+
+val lemma_ws_def_1: (b:Spec.SHA2.block_w) -> (t:Spec.SHA2.counter{16 <= t /\ t < 64}) -> Lemma
+  (Spec.SHA2.ws b t =
+    (let open Spec.SHA2 in
+     let t16 = ws b (t - 16) in
+     let t15 = ws b (t - 15) in
+     let t7  = ws b (t - 7) in
+     let t2  = ws b (t - 2) in
+     let s1 = _sigma1 t2 in
+     let s0 = _sigma0 t15 in
+     s1 +%^ (t7 +%^ (s0 +%^ t16))))
+#reset-options "--initial_fuel 1 --max_fuel 1 --z3rlimit 20"
+let lemma_ws_def_1 b t = ()
+
+
+#reset-options "--max_fuel 0 --max_ifuel 0 --z3rlimit 100"
+
+let lemma_modifies_0_is_modifies_1 (#a:Type) (h:HyperStack.mem) (b:buffer a{live h b}) : Lemma
+  (modifies_1 b h h) =
+  lemma_intro_modifies_1 b h h
+
